TraceSemantics.v
@@ -56,7 +56,6 @@ Inductive head_red__S: (trace__S * Stmt) -> (trace__S * Stmt) -> Prop :=
     head_red__S (t, <{ while b {s} }>) (t :: Cond b, <{s ; while b {s}}>)
 | head_red_loop_false__S: forall t b s,
     head_red__S (t, <{ while b {s} }>) (t :: Cond (BNot b), SSkip)
-(* I don't love these cases, they're a bit inelegant *)
 | head_red_seq__S: forall s t,
     head_red__S (t, <{skip ; s}>) (t, s)
 | head_red_par__S: forall t,
@@ -75,7 +74,6 @@ Inductive head_red__C (V0:Valuation): (trace__C * Stmt) -> (trace__C * Stmt) -> 
     head_red__C V0 (t, <{ if b {s1} {s2} }>) (t, if (Beval_t V0 t b) then s1 else s2)
 | head_red_loop__C: forall t b s,
     head_red__C V0 (t, <{while b {s}}>) (t, if (Beval_t V0 t b) then <{s ; while b {s}}> else SSkip)
-(* I don't love these cases, they're a bit inelegant *)
 | head_red_skip_seq__C: forall s t,
     head_red__C V0 (t, <{skip ; s}>) (t, s)
 | head_red_par__C: forall t,
@@ -114,7 +112,7 @@ Proof.
   - simpl in H1. apply andb_true_iff in H1. destruct H1.
     unfold Bapply_t in H. rewrite <- comp_subB in H. rewrite <- H2 in H.
     exists t0'. splits.
-    (* there's got to be a better way to do this...*)
+    (* manually unfolding the statement *)
     + assert (head_red__C V0 (t0', <{ if b {s'0}{s2} }>) (t0', if Beval_t V0 t0' b then s'0 else s2)) by constructor.
       unfold Beval_t in H3. rewrite H in H3. apply H3.
     + assumption.
@@ -123,7 +121,6 @@ Proof.
     apply negb_true_iff in H.
     unfold Bapply_t in H. rewrite <- comp_subB in H. rewrite <- H2 in H.
     exists t0'. splits.
-    (* there's got to be a better way to do this...*)
     + assert (head_red__C V0 (t0', <{ if b {s1}{s'0} }>) (t0', if Beval_t V0 t0' b then s1 else s'0)) by constructor.
       unfold Beval_t in H3. rewrite H in H3. apply H3.
     + assumption.
@@ -131,7 +128,6 @@ Proof.
   - simpl in H1. apply andb_true_iff in H1. destruct H1.
     unfold Bapply_t in H. rewrite <- comp_subB in H. rewrite <- H2 in H.
     exists t0'. splits.
-    (* there's got to be a better way to do this...*)
     + assert (head_red__C V0 (t0', <{ while b {s} }>) (t0', if Beval_t V0 t0' b then <{s ; while b {s}}> else SSkip)) by constructor.
       unfold Beval_t in H3. rewrite H in H3. apply H3.
     + assumption.
@@ -140,7 +136,6 @@ Proof.
     apply negb_true_iff in H.
     unfold Bapply_t in H. rewrite <- comp_subB in H. rewrite <- H2 in H.
     exists t0'. splits.
-    (* there's got to be a better way to do this...*)
     + assert (head_red__C V0 (t0', <{ while b {s} }>) (t0', if Beval_t V0 t0' b then <{s ; while b {s}}> else SSkip)) by constructor.
       unfold Beval_t in H3. rewrite H in H3. apply H3.
     + assumption.
